WIP: Try to make EchoServer actual work. There is a problem with the integers

io/case-study/Extract_ML.ml
@@ -7,54 +7,60 @@ let ml_openfile (file_name, flags, perm) : file_descr maybe =
   try
     let fd = Unix.openfile file_name flags (Z.to_int perm) in
     Inl fd ;
-  with err -> raise err; Inr err ;;
+  with err -> print_string "here1"; print_newline (); raise err; Inr err ;;
 
 let ml_read (fd, limit) : (FStar_Bytes.bytes * int) maybe =
-  try 
-    let buff = Bytes.make limit '\000' in
+  try
+    let (_, limit) : (file_descr * int) = Obj.magic (fd, (Stdint.Int32.of_int (256))) in
+    print_int limit;
+    print_newline ();
+    let buff = Bytes.make 256 '\000' in
     let c = Unix.read fd buff 0 limit in
     Inl ((Bytes.to_string buff), c) ;
-  with err -> raise err; Inr err ;;
+  with err -> print_string "here2"; print_newline (); raise err; Inr err ;;
 
 let ml_write (fd, message) : unit maybe =
   try 
     let byts = Bytes.of_string message in
     let _ = Unix.write fd byts 0 (Bytes.length byts) in
     Inl () ;
-  with err -> raise err; Inr err ;;
+  with err -> print_string "here3"; print_newline (); raise err; Inr err ;;
 
 let ml_close fd : unit maybe =
   try
     Unix.close fd;
     Inl () ;
-  with err -> raise err; Inr err ;; 
+  with err -> print_string "here4"; print_newline (); raise err; Inr err ;; 
 
 let ml_socket () : file_descr maybe =
   try
     print_string "Socket created\n";
     print_newline ();
     Inl (Unix.socket Unix.PF_INET Unix.SOCK_STREAM 0) ;
-  with err -> raise err; Inr err ;;
+  with err -> print_string "here5"; print_newline (); raise err; Inr err ;;
 
 let ml_setsockopt (socket, opt, value) : unit maybe =
   try
     Unix.setsockopt socket opt value;
     Inl () ;
-  with err -> raise err; Inr err ;;
+  with err -> print_string "here6"; print_newline (); raise err; Inr err ;;
 
 let ml_bind (socket, address, port) : unit maybe =
   try
-    Unix.bind socket (Unix.ADDR_INET(Unix.inet_addr_of_string "0.0.0.0", port));
+    let limit : int = Stdint.Int.of_int (256) in
+    print_int limit;
+    print_newline ();
+    Unix.bind socket (Unix.ADDR_INET(Unix.inet_addr_of_string address, port));
     print_string "Binded ...\n";
     print_newline ();
     Inl () ;
-  with err -> raise err; Inr err ;;
+  with err -> print_string "here7"; print_newline (); raise err; Inr err ;;
 
 let ml_setnonblock fd : unit maybe = 
   try
     Unix.set_nonblock fd;
     Inl () ;
-  with err -> raise err; Inr err ;;
+  with err -> print_string "here8"; print_newline (); raise err; Inr err ;;
 
 let ml_listen (fd, limit) : unit maybe = 
   try
@@ -62,17 +68,23 @@ let ml_listen (fd, limit) : unit maybe =
     print_newline ();
     Unix.listen fd limit;
     Inl () ;
-  with err -> raise err; Inr err ;;
+  with err -> print_string "here9"; print_newline (); raise err; Inr err ;;
 
 let ml_accept fd : Unix.file_descr maybe = 
   try
     let fd', _ = Unix.accept fd in
     Inl (fd') ;
-  with err -> raise err; Inr err ;;
+  with err -> print_string "here10"; print_newline (); raise err; Inr err ;;
 
 let ml_select (l1, l2, l3, t) : (lfds * lfds * lfds) maybe =
   try
     Inl (Unix.select l1 l2 l3 (100.0 /. 1000.0)) ;
-  with err -> raise err; Inr err ;;
+  with err -> print_string "here11"; print_newline (); raise err; Inr err ;;
 
 let ml_gettrace () : Free_IO.trace = []
+
+let console_log s =
+  print_string s;
+  print_string "\n";
+  print_newline ();
+  ()
